Improved naming a bit for functional extensionality

examples/metatheory/stlc_cbv_db_parsubst.fst
@@ -22,6 +22,7 @@ module StlcCbvDbParSubst
    is _more_ complex than the one in stlc_strongred.fst! *)
 
 open StlcStrongDbParSubst
+open FunctionalExtensionality
 
 val step : exp -> Tot (option exp)
 let rec step e =
@@ -159,8 +160,8 @@ let subst_gen_elam_aux x v y =
      else ())
 
 val subst_gen_elam_aux_forall : x:var -> v:exp{closed v} -> Lemma
-      (ensures (SubEqual (subst_elam (sub_beta_gen  x    v))
-                                     (sub_beta_gen (x+1) v)))
+      (ensures (FEq (subst_elam (sub_beta_gen  x    v))
+                                (sub_beta_gen (x+1) v)))
 let subst_gen_elam_aux_forall x v = admit()
 (* should follow from subst_gen_elam_aux and forall_intro *)
 
@@ -173,54 +174,6 @@ let subst_gen_elam x v t_y e' =
                                       (sub_beta_gen (x+1) v)  e';
   assert(subst_beta_gen x v (ELam t_y e')
            = ELam t_y (subst e' (subst_elam (sub_beta_gen x v))))
-
-(* [some comment that might help here]
-   NS: The trouble is that you need extensionality for this proof to go through. 
-   [snip]
-   A good way to solve this would be to use the same recipe
-   that is being used in partialmap.fst for set, map etc. 
-
-   -- Ideally, we would implement Map in the same style as Set, using
-       functions (rather than axioms).
-
-   -- Then, define Map.Equal to be extensional equality on maps, and
-       admit one axiom, i.e, Extensional, allowing extensional maps to
-       be treated as syntactically equal.
- 
-   -- Define type sub = Map.map var exp
-
-   -- Then, prove a lemma:
-        val subst_extensional: s1:sub -> s2:sub -> e:exp -> Lemma (ensures (Map.Equal s1 s2) ==> (subst e s1 = subst e s2))
-                                                                  [SMTPat [subst e s1; subst e s2])
-
-        let subst_extensional s1 s2 e = () //the proof should be trivial with the extensionality axiom
-
-   -- With this, your proof should just go through trivially.
-     
-      Be aware that you will really need that SMTPat. 
-      Let's look at the goal again:
-
-         EApp (subst e1 s1) (subst e2 s1) = EApp (subst e1 s2) (subst e2 s3) 
-
-      You really don't have a way to get your hands on s1, s2,
-      s3. These are terms that come up as Z3 tries to search for a
-      proof. Since you can't get your hands on it, you will not be
-      able to call subst_extensional yourself. The SMT pat lets solver
-      call it when it needs to.
-
-      It would be nice if you could get your hands on s1, s2, s3
-      somehow ... but I don't know of a way to do it at the moment.
-
-      One improvement: maybe you don't want subst_extensional
-      polluting the proof context at the top-level. You could instead
-      write something like:
-
-      val use_subst_extensional: unit -> Lemma (ensures (forall s1 s2 e.{:pattern subst e s1; subst e s2}
-                                                               (Map.Equal s1 s2) ==> (subst e s1 = subst e s2)))
-
-      And then call it just in the scope where you want the solver to make use of it.
-      
- *)
 
 val substitution_preserves_typing :
       x:var -> #e:exp -> #v:exp -> #t_x:typ -> #t:typ -> #g:env ->
