lib/ext.fst
@@ -1,8 +1,8 @@
-module Extensionality
-type arr (a:Type) (b:Type) = a -> Tot b
+module FunctionalExtensionality
+type efun (a:Type) (b:Type) = a -> Tot b
 
-opaque logic type Eq : #a:Type -> #b:Type -> arr a b -> arr a b -> Type =
-           fun (a:Type) (b:Type) (f:arr a b) (g:arr a b) -> (forall x. f x = g x)
+opaque logic type FEq : #a:Type -> #b:Type -> efun a b -> efun a b -> Type =
+           fun (a:Type) (b:Type) (f:efun a b) (g:efun a b) -> (forall x. f x = g x)
 
-assume Extensionality : forall (a:Type) (b:Type) (f: arr a b) (g: arr a b).
-                        {:pattern Eq #a #b f g} Eq #a #b f g <==> f=g
+assume Extensionality : forall (a:Type) (b:Type) (f: efun a b) (g: efun a b).
+                        {:pattern FEq #a #b f g} FEq #a #b f g <==> f=g
